Working towards showing bfs reachability lemma

examples/data_structures/graph/Graph.Search.fst
@@ -6,8 +6,10 @@ open FStar.Fin
 open Seq.Complements
 module C = FStar.Classical
 open Graph.Base
-open List.Complements
+module LC = List.Complements
 module N = Graph.NodeSet
+module M = FStar.Map
+module MC = Map.Complements
 
 let lemma_reachable_trans (#n:nat) (g:graph0 n) (n1 n2 n3:fin n)
  : Lemma (requires (reachable g n1 n2) /\ (reachable g n2 n3))
@@ -20,7 +22,7 @@ let lemma_reachable_trans (#n:nat) (g:graph0 n) (n1 n2 n3:fin n)
 
 
 
-let rec bfs (#n:nat) (g:graph0 n{no_parallel_edge g}) (s:nodeset n) (f:nodeset n)
+let rec bfs_aux (#n:nat) (g:graph0 n{no_parallel_edge g}) (s:nodeset n) (f:nodeset n)
  : Pure (nodeset n)
  (requires (True) 
   /\ N.disjoint s f)
@@ -31,13 +33,117 @@ let rec bfs (#n:nat) (g:graph0 n{no_parallel_edge g}) (s:nodeset n) (f:nodeset n
  | hd :: tl ->
   let cn = hd in
   let adj = g @^ cn in
-  let adj_unscene = L.filter (fun n -> L.mem n s = false && L.mem n f = false) adj in
-  noRepeats_filter (fun n -> L.mem n s = false && L.mem n f = false) adj;
+  let neither_in_s_nor_f n = not (L.mem n s) && not (L.mem n f) in
+  let adj_unscene = L.filter neither_in_s_nor_f adj in
+  LC.noRepeats_filter neither_in_s_nor_f adj;
   let s' = hd :: s in
   let f' = N.append tl adj_unscene in
   N.lemma_disjoint_append tl adj_unscene s';
-  noRepeats_length_lemma (s');
-  bfs g s' f'
+  LC.noRepeats_length_lemma (s');
+  bfs_aux g s' f'
+
+let bfs (#n:nat) (g:graph0 n{no_parallel_edge g}) (node : fin n) =
+  let adj = g @^ node in
+  let adj_unscene = L.filter (fun n -> not (n = node)) adj in
+  LC.noRepeats_filter (fun n -> not (n = node)) adj;
+  bfs_aux g [node] adj_unscene
+
+
+let decrease_clause (n:nat) (s:nodeset n) : nat = LC.noRepeats_length_lemma s ; n - L.length s
+
+let rec bfs_map_aux (#n:nat) (g:graph0 n{no_parallel_edge g}) (seen:nodeset n) (frntr:nodeset n) (parents:M.t (fin n) (fin n))
+ : Pure (nodeset n * M.t (fin n) (fin n))
+ (requires  N.disjoint seen frntr)
+ (ensures (fun p' -> True ))
+ (decreases (decrease_clause n seen))
+ = match frntr with
+ | [] -> seen, parents
+ | hd :: tl ->
+  let adj = g @^ hd in
+  let neither_in_s_nor_f n = not (L.mem n seen) && not (L.mem n frntr) in
+  let adj_unscene = L.filter neither_in_s_nor_f adj in
+  LC.noRepeats_filter neither_in_s_nor_f adj;
+  
+  let s' = hd :: seen in
+  let f' = N.append tl adj_unscene in
+  let p' = L.fold_left (fun acc i -> M.upd acc i hd) parents adj_unscene in
+
+  N.lemma_disjoint_append tl adj_unscene s';
+(*  noRepeats_length_lemma (s');  *)
+  bfs_map_aux g s' f' p'
 
 
 
+let rec lemma_bfs_map_pairing_aux (#n:nat) (g:graph0 n{no_parallel_edge g}) (seen:nodeset n) (frntr:nodeset n) (parents:M.t (fin n) (fin n))
+ : Lemma 
+   (requires N.disjoint seen frntr /\
+     (forall (x : fin n) . M.contains parents x ==>  is_in_graph (M.sel parents x) x g) /\
+   (forall (x: fin n) . L.mem x seen || L.mem x frntr <==> M.contains parents x))
+ 
+   (ensures N.disjoint seen frntr /\
+   (let s', p' = bfs_map_aux g seen frntr parents in (forall (x : fin n) . M.contains p' x ==>  is_in_graph (M.sel p' x) x g)))
+   (decreases (decrease_clause n seen))
+ = match frntr with
+ | [] -> admit()
+ | hd :: tl ->
+
+  let adj = g @^ hd in
+  let neither_in_s_nor_f n = not (L.mem n seen) && not (L.mem n frntr) in
+  let adj_unscene = L.filter neither_in_s_nor_f adj in
+  LC.noRepeats_filter neither_in_s_nor_f adj;
+  
+  let s' = hd :: seen in
+  let f' = N.append tl adj_unscene in
+  let p' = L.fold_left (fun acc i -> M.upd acc i hd) parents adj_unscene in
+  assume((forall (x: fin n) . L.mem x s' || L.mem x f'  <==> M.contains p' x));
+  assume(N.disjoint s' f');
+  assume((forall (x : fin n) . M.contains p' x ==>  is_in_graph (M.sel p' x) x g));
+  
+  lemma_bfs_map_pairing_aux g s' f' p'
+
+
+let rec lemma_bfs_map_pairing_aux2 (#n:nat) (g:graph0 n{no_parallel_edge g}) (seen:nodeset n) (frntr:nodeset n) (parents:M.t (fin n) (fin n)) (si : nodeset n) (fi : nodeset n) (pi:M.t (fin n) (fin n))
+ : Lemma 
+   (requires N.disjoint seen frntr /\ N.disjoint si fi /\ 
+   (forall (x : fin n) . M.contains parents x ==>  is_in_graph (M.sel parents x) x g) /\
+   (forall (x: fin n) . L.mem x seen || L.mem x frntr <==> M.contains parents x))
+   (ensures N.disjoint si fi /\ 
+   (let s', p' = bfs_map_aux g si fi pi in s' == seen /\ p' == parents /\(forall (x : fin n) . M.contains p' x ==>  is_in_graph (M.sel p' x) x g)))
+   (decreases (decrease_clause n seen))
+ = match frntr with
+ | [] -> admit()
+ | hd :: tl ->
+
+  let adj = g @^ hd in
+  let neither_in_s_nor_f n = not (L.mem n seen) && not (L.mem n frntr) in
+  let adj_unscene = L.filter neither_in_s_nor_f adj in
+  LC.noRepeats_filter neither_in_s_nor_f adj;
+  
+  let s' = hd :: seen in
+  let f' = N.append tl adj_unscene in
+  let p' = L.fold_left (fun acc i -> M.upd acc i hd) parents adj_unscene in
+(*
+  N.lemma_disjoint_append tl adj_unscene s';
+  MC.lemma_fold_upd1 parents adj_unscene (fun _ -> hd);
+
+  assert(forall (x : fin n) . L.mem x seen ==>  M.sel parents x == M.sel p' x);
+  assert(forall (x : fin n) . L.mem x seen ==>  is_in_graph (M.sel parents x) x g);
+  MC.lemma_fold_upd2 parents adj_unscene (fun _ -> hd);
+  MC.domain_lemma parents adj_unscene (fun _ -> hd);
+  assert(forall (x:fin n) . L.mem x adj ==> is_in_graph hd x g);
+  LC.filter_sublist neither_in_s_nor_f adj;
+  assert(forall (x:fin n) . L.mem x adj_unscene ==>  L.mem x adj);
+  assert(forall (x:fin n) . L.mem x adj_unscene ==> is_in_graph hd x g);
+  assert(forall (x : fin n) . L.mem x adj_unscene ==>  is_in_graph (M.sel p' x) x g);
+  assert(forall (x : fin n) . L.mem x seen ==>  is_in_graph (M.sel p' x) x g);
+
+  MC.domain_lemma2 parents adj_unscene (fun _ -> hd);
+  assert(forall (x : fin n) . L.mem x seen || L.mem x adj_unscene ==> M.contains p' x);
+  
+  assert(forall (x : fin n) . M.contains p' x ==>  is_in_graph (M.sel p' x) x g);
+*)
+  assume((forall (x: fin n) . L.mem x s' || L.mem x f'  <==> M.contains p' x));
+  assume(N.disjoint s' f');
+  assume((forall (x : fin n) . M.contains p' x ==>  is_in_graph (M.sel p' x) x g));
+  
+  lemma_bfs_map_pairing_aux2 g s' f' p' si fi pi
